share/pulse/examples/parallel/DomainsPoolAlive.fsti
@@ -1,0 +1,916 @@
+module DomainsPoolAlive
+
+open Pulse.Lib.Pervasives
+module Lock = Pulse.Lib.SpinLock
+module HR = Pulse.Lib.HigherReference
+module M = Pulse.Lib.GhostMonotonicReference
+module L = FStar.List.Tot.Base
+
+
+module GR = Pulse.Lib.GhostReference
+
+open SingleGhostTask
+open GhostTaskQueue
+
+(* Pool: ghost_mono_ref, counter, task queue, lock, invariant... *)
+
+let task_queue: Type0 = list task
+
+(* also ghost queue? *)
+val mono_queue_ref: Type0
+val mono_queue: Type0 (* not 0? *)
+
+let link (l: mono_list) (q: task_queue) (c: int): prop
+= (count_ongoing l == c /\ get_actual_queue l == q)
+
+
+let if_then_else (b: bool) (thn: vprop) (els: vprop): vprop
+= if b then thn else els
+
+let lock_thn (l: mono_list) q c: vprop
+= (exists* vq vc. pts_to q vq ** pts_to c vc ** pure (link l vq vc))
+
+let lock_els l status_pool: vprop
+= (pure (link l [] 0) ** (exists* f1. pts_to status_pool #f1 false))
+(* maybe we'll need some permission to the ghost_mono_ref? maybe not *)
+
+
+let lock_pool
+  (status_pool: ref bool)
+  (q: ref task_queue)
+  (c: ref int)
+  (r: ghost_mono_ref)
+: vprop
+= (exists* sp l. pts_to status_pool #one_half sp ** M.pts_to r one_half l
+  ** (if_then_else sp (lock_thn l q c) (lock_els l status_pool)))
+
+let x = ()
+
+let pool = (status_pool: ref bool
+  & q: ref task_queue
+  & c: ref int
+  & ri: (r:ghost_mono_ref & inv (inv_ghost_queue r))
+  & Lock.lock (lock_pool status_pool q c ri._1))
+
+let mk_pool (status_pool: ref bool) (q: ref task_queue)
+  (c: ref int) (ri: (r:ghost_mono_ref & inv (inv_ghost_queue r)))
+  (lock: Lock.lock (lock_pool status_pool q c ri._1)): pool
+= (| status_pool, q, c, ri, lock |)
+
+let pool_alive (f: perm) (p: pool): vprop // f/2 permission to the ghost bool ref, true
+= pts_to p._1 #(half_perm f) true
+
+
+let locked_pool (p: pool): vprop =
+  lock_pool p._1 p._2 p._3 p._4._1
+
+```pulse
+ghost fn elim_if_then
+(b: bool) (thn: vprop) (els: vprop)
+requires if_then_else b thn els ** pure b
+ensures thn
+{
+  rewrite if_then_else b thn els as thn
+}
+```
+
+
+
+//#push-options "--print_implicits"
+```pulse
+ghost fn
+unfold_lock_pool_alive (#f: perm) (pl: pool)
+requires pool_alive f pl ** locked_pool pl
+//requires lock_pool pl._1 pl._2 pl._3 pl._4._1 ** pool_alive f pl
+ensures pool_alive f pl ** (exists* sp l. pts_to pl._1 #one_half sp ** M.pts_to pl._4._1 one_half l **
+  (exists* vq vc. pts_to pl._2 vq ** pts_to pl._3 vc ** pure (link l vq vc)))
+{
+  unfold locked_pool pl;
+  unfold lock_pool;
+  unfold pool_alive f pl;
+  with sp gq. assert (pts_to pl._1 #one_half sp ** M.pts_to pl._4._1 one_half gq);
+  pts_to_injective_eq pl._1;
+  fold pool_alive f pl;
+  elim_if_then _ _ _;
+  unfold lock_thn; //_ pl._2 pl._3;
+  ()
+}
+```
+
+```pulse
+ghost fn
+fold_lock_pool_alive (#f: perm) (pl: pool)
+requires pool_alive f pl ** (exists* sp l. pts_to pl._1 #one_half sp ** M.pts_to pl._4._1 one_half l **
+  (exists* vq vc. pts_to pl._2 vq ** pts_to pl._3 vc ** pure (link l vq vc)))
+ensures pool_alive f pl ** locked_pool pl
+//requires lock_pool pl._1 pl._2 pl._3 pl._4._1 ** pool_alive f pl
+{
+  admit()
+  (*
+  unfold locked_pool pl;
+  unfold lock_pool;
+  unfold pool_alive f pl;
+  with sp gq. assert (pts_to pl._1 #one_half sp ** M.pts_to pl._4._1 one_half gq);
+  pts_to_injective_eq pl._1;
+  fold pool_alive f pl;
+  elim_if_then _ _ _;
+  unfold lock_thn; //_ pl._2 pl._3;
+  ()
+  *)
+}
+```
+(*
+TODO: Actually launch workers...
+*)
+```pulse
+fn setup_pool (n: int{n >= 1})
+  requires emp
+  returns pl: pool
+  ensures pool_alive full_perm pl
+{
+  let ri: (r: ghost_mono_ref & inv (inv_ghost_queue r)) = create_ghost_queue ();
+
+  let status_pool: ref bool = alloc true;
+  share2 status_pool;
+
+  let q: ref task_queue = alloc #task_queue [];
+  let c: ref int = alloc 0;
+
+  assert (pts_to q [] ** pts_to c 0 ** pure (link [] [] 0));
+  assert (exists* vq vc. pts_to q vq ** pts_to c vc ** pure (link [] vq vc));
+  fold lock_thn [] q c;
+  fold (if_then_else true (lock_thn [] q c) (lock_els [] status_pool));
+
+  fold (lock_pool status_pool q c ri._1);
+  let lock = Lock.new_lock (lock_pool status_pool q c ri._1);
+
+  let pl: pool = mk_pool status_pool q c ri lock;
+  rewrite each status_pool as pl._1;
+  fold pool_alive full_perm pl;
+  pl
+}
+```
+
+(*
+probably this lock needs to be in the task queue?
+*)
+
+type handler (pl: pool) (post: vprop) =
+  t:task & (pos:nat) & certificate pl._4._1 t pos //& Lock.lock (lock_task t)//(exists* v. pts_to t._4 #one_half v)
+
+let mk_handler_pure (pl: pool) (post: vprop) (t: task) (pos: nat) (certif: certificate pl._4._1 t pos)
+  //(lock: Lock.lock (lock_task t))
+  : handler pl post
+= (| t, pos, certif |)
+
+```pulse
+fn mk_handler
+(pl: pool) (post: vprop) (t: task) 
+(res: (pos:nat & certificate pl._4._1 t pos))
+//(pos: nat) (certif: certificate pl._4._1 t pos)
+requires GR.pts_to t._5 #one_half false
+returns h: handler pl post
+ensures GR.pts_to h._1._5 #one_half false
+{
+  //fold lock_task t;
+  //let lock = Lock.new_lock (lock_task t);
+  let h: handler pl post = mk_handler_pure pl post t res._1 res._2;
+  rewrite each t as h._1;
+  h
+}
+```
+  
+  //(lock: Lock.lock (exists* v. pts_to t._4 #one_half v)): handler pl post
+
+(*
+      GR.pts_to (Mkdtuple5?._5 t) (reveal (hide false)) ** 
+      pts_to (Mkdtuple5?._4 t) (reveal (hide false)) ** 
+    *)
+
+(*
+TODO:
+ASSUMING!
+*)
+(*
+val read_ghost_mono_ref (#a:Type) (#p:Preorder.preorder a) (#f: perm)
+    (r:M.ref a p)
+  : stt_atomic a #Unobservable emp_inames
+  (exists* v. M.pts_to r f v) (fun vv -> M.pts_to r f vv)
+  (* How wrong is this? *)
+  *)
+val read_ghost_mono_ref (#a:Type) (#p: Preorder.preorder a) (r:M.ref a p) (#n:erased a) (#p:perm)
+  : stt a
+        (M.pts_to r p n)
+        (fun x -> M.pts_to r p n ** pure (reveal n == x))
+
+let enqueue_add_task_get_actual (l: mono_list) (t: task) (vq: task_queue) (vc: int):
+  Lemma (requires link l vq vc)
+  (ensures link (enqueue_todo l t)._1 (t::vq) vc)
+= ()
+
+```pulse
+ghost fn pulse_enqueue_add_task_get_actual (l: mono_list) (t: task) (vq: task_queue) (vc: int)
+requires pure (link l vq vc)
+ensures pure (link (enqueue_todo l t)._1 (t::vq) vc)
+{
+  ()
+}
+```
+
+
+
+val assume_prop (p: prop):
+stt unit emp (fun () -> pure p)
+
+#push-options "--print_implicits"
+```pulse
+fn async #pre #post #f (pl: pool) (ta: (unit -> stt unit pre (fun () -> post)))
+  requires pool_alive f pl ** pre
+  returns h: handler pl post
+  // returns pr: promise pl unit post, or handler
+  ensures pool_alive f pl ** GR.pts_to h._1._5 #one_half false
+  // ** pledge (task_done pr) post
+{
+  let ti: (t: task & inv (guarded_inv t._2 post)) = create_task ta;
+  let t = ti._1;
+  let itask: inv (guarded_inv t._2 post) = ti._2;
+
+  let status_pool: ref bool = pl._1;
+  let q: ref task_queue = pl._2;
+  let c: ref int = pl._3;
+  let r: ghost_mono_ref = pl._4._1;
+  let i: inv (inv_ghost_queue r) = pl._4._2;
+  let lock = pl._5;
+
+  Lock.acquire pl._5;
+  //show_proof_state;
+  rewrite (lock_pool (Mkdtuple5?._1 pl) (Mkdtuple5?._2 pl) (Mkdtuple5?._3 pl) (Mkdtuple2?._1 (Mkdtuple5?._4 pl)))
+    as locked_pool pl;//(lock_pool status_pool q c r);
+  unfold_lock_pool_alive pl;
+
+  rewrite each pl._1 as status_pool;
+  rewrite each pl._2 as q;
+  rewrite each pl._3 as c;
+  rewrite each pl._4._1 as r;
+  rewrite each pl._4._2 as i;
+  rewrite each pl._5 as lock;
+  rewrite each ti._1 as t;
+
+  //with ll. assert (M.pts_to r one_half ll);
+  let l: mono_list = read_ghost_mono_ref r;
+  let ll: mono_list = (enqueue_todo l t)._1;
+  with vq vc. assert (pts_to q vq ** pts_to c vc);
+  let vq_: task_queue = !q;
+  let vq': task_queue = Prims.Cons #task t vq_;
+  assert pure (link l vq vc);
+  assert pure (link ll vq' vc);
+
+  rewrite each ti._1 as t;
+  //share2 t._4._1;
+  assert GR.pts_to t._5 #full_perm false;
+  GR.share2 t._5;
+  assert GR.pts_to t._5 #one_half false ** GR.pts_to t._5 #one_half false;
+  let res: (pos:nat & certificate r t pos) = add_todo_task_to_queue r i t l;
+  //assert M.pts_to r one_half (enqueue_todo l t)._1;
+
+  assert pts_to q (reveal vq);
+  q := vq'; //(enqueue_todo l t)._1;
+  assert pure (link ll vq' vc);
+  assert pool_alive f pl;
+  with sp. assert pts_to status_pool #one_half sp ** M.pts_to r one_half ll;
+
+  assert pool_alive f pl;
+  rewrite each status_pool as pl._1;
+  rewrite each q as pl._2;
+  rewrite each c as pl._3;
+  rewrite each r as pl._4._1;
+  assert (exists* sp l. pts_to pl._1 #one_half sp ** M.pts_to pl._4._1 one_half l **
+  (exists* vq vc. pts_to pl._2 vq ** pts_to pl._3 vc ** pure (link l vq vc)));
+  fold_lock_pool_alive pl;
+  rewrite (locked_pool pl) as lock_pool pl._1 pl._2 pl._3 pl._4._1;
+  Lock.release pl._5;
+  let h: handler pl post = mk_handler pl post t res;
+  h
+}
+```
+
+```pulse
+ghost fn get_task_done (t: task) (f: perm)
+requires pts_to t._4._1 #f true
+ensures task_done t
+{
+  fold task_done t
+}
+```
+
+```pulse
+ghost fn close_lock_task (bdone: ref bool) (f: perm) (v: bool)
+requires pts_to bdone #f v ** pure (if not v then f == one_half else true)
+ensures lock_task bdone
+{
+  fold lock_task bdone;
+}
+```
+
+(*
+pool_alive is currently not necessary, because we never deallocate the reference where we say whether we're done...
+*)
+#pop-options
+```pulse
+fn await (#pl: pool) (#post: vprop) (h: handler pl post)
+  requires pool_alive f pl
+  ensures pool_alive f pl ** task_done h._1
+{
+  let mut task_is_done = false;
+  rewrite emp as (if false then task_done h._1 else emp);
+  let bdone: ref bool = h._1._4._1;
+  let lock: Lock.lock (lock_task bdone) = h._1._4._2;
+  while (let d = !task_is_done; not d)
+    invariant b. (exists* d. pts_to task_is_done d ** pure (b == not d) ** (if d then task_done h._1 else emp)
+    //** pure (bdone == h._1._4._1) 
+    )
+  {
+    with d. assert pts_to task_is_done d;
+    Lock.acquire lock;
+    rewrite lock_task bdone
+      as (exists* v f. pts_to bdone #f v ** pure (if not v then f == one_half else true));
+    with v f. assert pts_to bdone #f v ** pure (if not v then f == one_half else true);
+    let vdone: bool = !bdone;
+    task_is_done := vdone;
+    rewrite (match reveal d <: bool with | true -> task_done (Mkdtuple3?._1 h) | _ -> emp) as emp;
+    if (vdone) {
+      share bdone;
+      assert pure (bdone == h._1._4._1);
+      rewrite (pts_to bdone #(half_perm f) v) as pts_to h._1._4._1 #(half_perm f) true;
+      assert pts_to h._1._4._1 #(half_perm f) true;
+      get_task_done h._1 (half_perm f);
+      rewrite task_done h._1 as (if true then task_done h._1 else emp);
+      close_lock_task bdone (half_perm f) true;
+      Lock.release h._1._4._2;
+      assert pts_to task_is_done true;
+      assert (pts_to task_is_done true ** (if true then task_done h._1 else emp));
+      ()
+    }
+    else {
+      rewrite emp as (if false then task_done h._1 else emp);
+      close_lock_task bdone f false;
+      Lock.release h._1._4._2;
+      ()
+    }
+  };
+  with d. assert pts_to task_is_done d;
+  assert (if d then task_done h._1 else emp) ** pure (false = not d);
+  elim_if_then d _ emp;
+  //rewrite (if d then task_done h._1 else emp) as task_done h._1;
+  ()
+}
+```
+
+```pulse
+ghost fn intro_if_then
+(b: bool) (thn: vprop) (els: vprop)
+requires thn ** pure b
+ensures if_then_else b thn els
+{
+  fold if_then_else b thn els;
+}
+```
+
+```pulse
+ghost fn
+close_lock_thn (q: ref task_queue) (c: ref int) (l: mono_list{~(get_actual_queue l == [])}) (vq: task_queue) (vc: int)
+requires pts_to q vq ** pts_to c (vc + 1) ** pure (link l vq vc)
+ensures lock_thn (pop_todo_task l)._2 q c
+{
+  admit()
+}
+```
+
+(*
+val pts_to_injective_eq (#a:_)
+                        (#p #q:_)
+                        (#v0 #v1:a)
+                        (r:ref a)
+  : stt_ghost unit
+      (pts_to r #p v0 ** pts_to r #q v1)
+      (fun _ -> pts_to r #p v0 ** pts_to r #q v1 ** pure (v0 == v1))
+*)
+
+#push-options "--print_implicits"
+
+(* Not sure if useful... *)
+```pulse
+fn write_done (t: task)
+  requires pts_to t._4._1 #one_half false
+  ensures pts_to t._4._1 #one_half true
+{
+  let bdone: ref bool = t._4._1;
+  let lock: Lock.lock (lock_task bdone) = t._4._2;
+  rewrite each t._4._1 as bdone;
+  assert pts_to bdone #one_half false;
+  Lock.acquire lock;
+  unfold lock_task bdone;
+  with f v. assert (pts_to bdone #f v ** pure (if not v then f == one_half else true));
+  pts_to_injective_eq bdone;
+  rewrite each f as one_half;
+  gather2 bdone;
+  bdone := true;
+  share2 bdone;
+  fold lock_task bdone;
+  Lock.release lock;
+  rewrite each bdone as t._4._1;
+  ()
+}
+```
+
+let perform_task (t: task):
+stt unit
+  (GR.pts_to t._1 #one_half true ** GR.pts_to t._2 #one_half false)
+  (fun () -> GR.pts_to t._1 #one_half false ** GR.pts_to t._2 #one_half true)
+= t._3 ()
+
+#pop-options
+
+(* TODO: How do I make this unobservable? *)
+
+```pulse
+ghost fn fold_lock_pool (sp: bool) (l: mono_list) (q: ref task_queue) (c: ref int) (status_pool: ref bool) (t: task)
+requires if_then_else sp (lock_thn l q c) (lock_els l status_pool) ** pts_to status_pool #one_half sp ** M.pts_to r one_half l
+ensures lock_pool status_pool q c r
+{
+  fold lock_pool status_pool q c r
+}
+```
+
+#push-options "--print_implicits"
+
+(*
+Ideally, the following would be unobservable
+--> Need to be able to read in unobservable
+*)
+```pulse
+fn
+prove_contradiction (r: ghost_mono_ref)
+(t: task) (pos: nat)
+(w: certificate r t pos)
+(q: ref task_queue) (c: ref int) (i: inv (inv_ghost_queue r))
+requires pts_to t._4._1 #one_half false ** lock_pool status_pool q c r
+ensures pts_to t._4._1 #one_half false ** (exists* l. pts_to status_pool #one_half true ** M.pts_to r one_half l ** lock_thn l q c)
+{
+  unfold lock_pool;
+  with sp l. assert pts_to status_pool #one_half sp ** M.pts_to r one_half l ** if_then_else sp (lock_thn l q c) (lock_els l status_pool);
+
+  let pool_alive: bool = !status_pool;
+  assert pure (pool_alive == sp);
+
+  if (pool_alive) {
+    elim_if_then sp _ _;
+    ()
+  }
+  else {
+
+    //assert pure (reveal sp == True);
+    let ll: mono_list = read_ghost_mono_ref r;
+    // Derive contradiction
+    rewrite (if_then_else (reveal sp) (lock_thn (reveal l) q c) (lock_els (reveal l) status_pool))
+      as lock_els (reveal l) status_pool;
+    unfold lock_els;
+    assert pure (link (reveal l) [] 0);
+    assert pure (link ll [] 0);
+    //M.recall #mono_list #one_half #is_mono_suffix (task_in_queue t pos) r ll w;
+    get_task_in_queue r one_half ll t pos w;
+    assert pure (task_in_queue t pos ll);
+    get_free_task_done t pos r i ll;
+
+    fold lock_els l status_pool;
+    rewrite (lock_els (reveal l) status_pool) as
+      (if_then_else sp (lock_thn (reveal l) q c) (lock_els (reveal l) status_pool));
+    assert (if_then_else (reveal sp) (lock_thn (reveal l) q c) (lock_els (reveal l) status_pool) ** pts_to t._4._1 #one_half false);
+    fold_lock_pool sp l q c status_pool t;
+    unfold task_done;
+    with f. assert (pts_to t._4._1 #f true);
+    gather t._4._1;
+    assert pure false;
+    
+    rewrite (pts_to #bool t._4._1 #(sum_perm (reveal #perm f) one_half) true ** lock_pool status_pool q c r)
+      as (pts_to t._4._1 #one_half false ** (exists* l. pts_to status_pool #one_half true ** M.pts_to r one_half l ** lock_thn l q c));
+
+    ()
+  }
+}
+```
+
+(*
+let rec close_task_bis_lemma
+(t: task) (pos: nat)
+(l: mono_list{task_in_queue t pos l /\ L.length l >= 1}):
+Lemma (ensures get_actual_queue (close_task_bis t pos l) == get_actual_queue l /\ count_ongoing (close_task_bis t pos l) = count_ongoing l - 1)
+= 
+let (t', s)::q = l in
+if pos + 1 = L.length l
+  then (assume (s = Ongoing); ())
+  //(t', Done)::q // if s is not Ongoing, then we have too much permission
+  else close_task_bis_lemma t pos q
+*)
+
+
+(*
+```pulse
+fn decrease_counter
+(t: task) (pos: nat)
+(l: mono_list{task_in_queue t pos l /\ L.length l >= 1})
+(q: ref task_queue) (c: ref int)
+requires lock_thn l q c
+ensures lock_thn (close_task_bis t pos l) q c
+{
+  unfold lock_thn l q c;
+  with vq' vc'. assert (pts_to q vq' ** pts_to c vc' ** pure (link l vq' vc'));
+  let vc: int = !c;
+  c := vc - 1;
+  close_task_bis_lemma t pos l;
+  fold lock_thn (close_task_bis t pos l) q c;
+  ()
+}
+```
+*)
+
+
+#pop-options
+
+val drop_task_done (t: task): stt_ghost unit (task_done t) (fun () -> emp)
+
+```pulse
+fn worker (pl: pool)
+requires emp
+ensures emp
+{
+  let mut r_working = true;
+  let status_pool: ref bool = pl._1;
+  let q: ref task_queue = pl._2;
+  let c: ref int = pl._3;
+  let r: ghost_mono_ref = pl._4._1;
+  let i: inv (inv_ghost_queue r) = pl._4._2;
+  let lock: Lock.lock (lock_pool status_pool q c r) = pl._5;
+ 
+  while (let working = !r_working; working)
+    invariant b. (exists* w. pts_to r_working w ** pure (b == w))
+  {
+    Lock.acquire lock;
+    unfold lock_pool status_pool q c r;
+    with sp_ l_. assert (pts_to status_pool #one_half sp_ ** M.pts_to r one_half l_ ** (if_then_else sp_ (lock_thn l_ q c) (lock_els l_ status_pool)));
+    let alive: bool = !status_pool;
+    if (alive) {
+      elim_if_then sp_ _ _;
+      unfold lock_thn l_ q c;
+      with vq_ vc_. assert pts_to q vq_ ** pts_to c vc_ ** pure (link l_ vq_ vc_);
+      let vq: task_queue = !q;
+
+      if (L.length vq > 0) {
+        let vc: int = !c;
+        let l: mono_list = read_ghost_mono_ref r;
+        let ll: mono_list = (pop_todo_task l)._2;
+
+        // 1. pop the task and increase counter
+        c := vc + 1;
+        let w: (pos:nat & certificate r (pop_todo_task l)._1 pos) = pop_task_ghost r i l;
+        rewrite each (pop_todo_task l)._2 as ll;
+        close_lock_thn q c l vq_ vc_;
+        intro_if_then sp_ (lock_thn (pop_todo_task l)._2 q c) (lock_els (pop_todo_task l)._2 status_pool);
+        rewrite each (pop_todo_task l)._2 as ll;
+        fold lock_pool status_pool q c r;
+        Lock.release lock;
+
+        // 2. perform the task
+        let t: task = (pop_todo_task l)._1;
+        let pos: nat = w._1;
+        let certif: certificate r t pos = w._2;
+        rewrite each (pop_todo_task l)._1 as t;
+
+        perform_task t;
+
+        // 3. conclude, and decrease counter
+        Lock.acquire lock;
+        unfold ongoing_condition;
+        assert pts_to t._4._1 #one_half false;
+        prove_contradiction r t pos certif q c i;
+
+        let l: mono_list = read_ghost_mono_ref r;
+        with ll. assert pts_to status_pool #one_half true ** M.pts_to r one_half ll ** lock_thn ll q c;
+        rewrite each (reveal ll) as l;
+        get_task_in_queue r one_half l t pos certif;
+
+        assert pure (task_in_queue t pos l);
+        let bdone: ref bool = t._4._1;
+        rewrite each t._4._1 as bdone;
+        let ltask: Lock.lock (lock_task bdone) = t._4._2;
+
+        Lock.acquire ltask;
+        unfold lock_task bdone;
+        with f v. assert (pts_to bdone #f v ** pure (if not v then f == one_half else true));
+        pts_to_injective_eq bdone;
+        rewrite each bdone as t._4._1;
+        fold ongoing_condition t;
+        //show_proof_state;
+        //rewrite (pts_to bdone #one_half false ** GR.pts_to t._5 #one_half false) as ongoing_condition t;
+        rewrite each f as one_half;
+        conclude_task t pos r i l;
+        rewrite each t._4._1 as bdone;
+        fold lock_task bdone;
+        Lock.release ltask;
+
+(*
+      task_done t ** 
+      pts_to r_working (reveal w) ** 
+      pts_to status_pool true ** 
+      lock_thn l q c ** 
+      M.pts_to r one_half (close_task_bis t pos l)
+*)
+        //show_proof_state;
+        //decrease_counter t pos l q c;
+ unfold lock_thn l q c;
+  with vq' vc'. assert (pts_to q vq' ** pts_to c vc' ** pure (link l vq' vc'));
+  let vc: int = !c;
+  c := vc - 1;
+  //close_task_bis_lemma t pos l;
+  fold lock_thn (close_task_bis t pos l) q c;
+  
+        intro_if_then true (lock_thn (close_task_bis t pos l) q c) (lock_els (close_task_bis t pos l) status_pool);
+        fold lock_pool status_pool q c r;
+
+        drop_task_done t;
+        Lock.release lock
+      }
+      else {
+        (* nothing to do *)
+        fold lock_thn l_ q c;
+        intro_if_then sp_ (lock_thn l_ q c) (lock_els l_ status_pool);
+        fold lock_pool status_pool q c r;
+        Lock.release lock
+      }
+    }
+    else {
+      r_working := false; // the pool has been deallocated, the worker can stop its job
+      fold lock_pool status_pool q c r;
+      Lock.release lock
+    }
+  };
+  ()
+}
+```
+
+let x = ()
+
+```pulse
+fn join_pool (#f: perm) (pl: pool)
+requires pool_alive f pl // takes a pledge
+ensures pool_alive f pl
+{
+  admit()
+}
+```
+
+```pulse
+fn teardown_pool (#f: perm) (pl: pool)
+  requires pool_alive f pl // ** pledge (pool_done pl) (pool_alive (1-f) p)
+  ensures pool_done pl
+{
+  admit()
+}
+```
+
+(*
++ there's an invariant somewhere that proves post of Some x
+*)
+
+(* where are stored the invariant? *)
+(* in the certificate... *)
+
+
+(*
+let small_inv (r: erased (ghost_mono_ref task_elem)) (q: list task_elem) (c: int): vprop 
+= exists_ (fun l -> pts_to_ghost_queue_half r l **
+  tasks_res_own l one_half **
+  pure (count_ongoing l = c /\ get_actual_queue l == q)
+  ** (if c = 0 && L.length q = 0 then deadline r
+  else pts_to_ghost_queue_half r l ** tasks_res_own l one_quart)
+*)
+
+(*
+could be:
+
+
+*)
+
+```pulse
+ghost fn open_lock_pool_alive
+(p: pool) (f: perm)
+requires pool_alive f p ** locked_pool p
+ensures pool_alive f p ** (exists* gq q c.
+  pts_to p._1 #one_half true ** pts_to_mono_queue p._4 full_perm gq ** HR.pts_to p._2 q ** pts_to p._3 c ** pure (link gq q c))
+{
+  unfold locked_pool p;
+  unfold lock_pool;
+  unfold pool_alive f p;
+
+  with sp gq. assert (pts_to p._1 #one_half sp ** pts_to_mono_queue p._4 one_half gq);
+ //** (if sp then (pts_to_mono_queue p._4 one_half gq ** (exists* q c. HR.pts_to p._2 q ** pts_to p._3 c ** inv gq q c))
+  //  else (inv gq [] 0 ** (exists* f1 f2. pts_to p._1 #f1 sp ** pts_to_mono_queue p._4 f2 gq))));
+  
+  pts_to_injective_eq p._1;
+
+  assert pure (sp);
+
+  elim_if_then sp _ _;
+(*
+  rewrite (if sp then (lock_thn gq p._4 p._2 p._3) else (lock_els gq p._1 p._4))
+    as (if true then (lock_thn gq p._4 p._2 p._3) else (lock_els gq p._1 p._4));
+
+
+  rewrite (if true then (lock_thn gq p._4 p._2 p._3) else (lock_els gq p._1 p._4))
+    as (lock_thn gq p._4 p._2 p._3);
+    *)
+
+  unfold lock_thn;
+
+
+  with q c. assert (HR.pts_to p._2 q ** pts_to p._3 c ** pure (link gq q c));
+  gather2_mono_queue p._4;
+
+  fold pool_alive f p;
+  ()
+}
+```
+
+#push-options "--print_implicits"
+
+```pulse
+ghost fn close_lock_pool_alive
+(p: pool) (f: perm)
+requires (exists* gq q c.
+  pts_to p._1 #one_half true ** pts_to_mono_queue p._4 full_perm gq ** HR.pts_to p._2 q ** pts_to p._3 c ** pure (link gq q c))
+ensures locked_pool p
+{
+  let status_pool = p._1;
+  with gq. assert (pts_to p._1 #one_half true ** pts_to_mono_queue p._4 full_perm gq);
+  rewrite each p._1 as status_pool;
+  // ** HR.pts_to p._2 q ** pts_to p._3 c ** inv gq q c);
+  share2_mono_queue p._4;
+
+  assert (pts_to status_pool #one_half true ** pts_to_mono_queue p._4 one_half gq);
+  //assert (pts_to_mono_queue p._4 one_half gq ** HR.pts_to p._2 q ** pts_to p._3 c ** inv gq q c);
+
+  //rewrite (pts_to_mono_queue p._4 one_half gq ** HR.pts_to p._2 q ** pts_to p._3 c ** inv gq q c)
+  //as (pts_to_mono_queue p._4 one_half gq ** (exists* q c. HR.pts_to p._2 q ** pts_to p._3 c ** inv gq q c));
+
+  //fold (if_then_else true (pts_to_mono_queue p._4 one_half gq ** (exists* q c. HR.pts_to p._2 q ** pts_to p._3 c ** inv gq q c))
+   //   (inv gq [] 0ghost_queue ** (exists* f1 f2. pts_to p._1 #f1 true ** pts_to_mono_queue p._4 f2 gq)));
+   fold lock_thn;
+
+intro_if_then true (lock_thn gq p._4 p._2 p._3) (lock_els gq status_pool p._4);
+
+assert (exists* gq. pts_to status_pool #one_half true ** pts_to_mono_queue p._4 one_half gq
+  ** (if_then_else true (lock_thn gq p._4 p._2 p._3) (lock_els gq status_pool p._4)));
+
+assert (pts_to status_pool #one_half true);
+//with sp. assert pts_to p._1 #one_half sp;
+//rewrite (pts_to p._1 #one_half true) as (exists* sp. pts_to p._1 #one_half sp);
+//assert (exists* sp. pts_to p._1 #one_half sp);
+assert (exists* sp gq. pts_to status_pool #one_half sp ** pts_to_mono_queue p._4 one_half gq);
+
+ fold lock_pool status_pool p._2 p._3 p._4;
+  (*
+pts_to status_pool #one_half sp
+
+  *)
+  
+  //fold lock_pool p._1 p._2 p._3 p._4;
+
+(*
+    assert (exists* sp gq. pts_to p._1 #one_half sp ** pts_to_mono_queue p._4 one_half gq
+  ** if_then_else sp (pts_to_mono_queue p._4 one_half gq **
+      (exists* q c. HR.pts_to p._2 q ** pts_to p._3 c ** inv gq q c))
+    (inv gq [] 0 ** (exists* f1 f2. pts_to p._1 #f1 sp ** pts_to_mono_queue p._4 f2 gq)));
+
+
+  assert (exists* sp. pts_to p._1 (reveal sp));
+
+  show_proof_state;
+  fold lock_pool p._1 p._2 p._3 p._4;
+  *)
+
+  
+//  with sp. assert (pts_to p._1 (reveal sp));
+
+(*
+  rewrite (pts_to p._1 sp) as (pts_to p._1 (reveal sp));
+
+  fold locked_pool p;
+  *)
+
+
+  //as (if_then_else sp (pts_to_mono_queue p._4 one_half gq ** (exists* q c. HR.pts_to p._2 q ** pts_to p._3 c ** inv gq q c))
+   //   (inv gq [] 0 ** (exists* f1 f2. pts_to p._1 #f1 sp ** pts_to_mono_queue p._4 f2 gq)));
+
+  //rewrite (pts_to_mono_queue p._4 one_half gq ** HR.pts_to p._2 q ** pts_to p._3 c ** inv gq q c)
+  //fold locked_pool p;
+
+  //rewrite (pts_to p._1 #one_half true ** pts_to_mono_queue p._4 one_half gq **
+  //(pts_to_mono_queue p._4 one_half gq ** HR.pts_to p._2 q ** pts_to p._3 c ** inv gq q c))
+  //as lock_pool p;
+
+
+  admit()
+}
+```
+
+
+
+
+
+let x = ()
+
+let deadline (p: pool): vprop
+= exists* f gq. pts_to_mono_queue p._4 f gq ** inv gq [] 0
+
+
+
+val certificate (p:pool) (t: task_elem) (pos: nat): Type0
+let secret_certificate (p: pool) (t: task_elem): Type0 = (pos: nat & certificate p t pos)
+
+//val deadline (p: pool): vprop // ghost bool ref, false
+
+val duplicate_deadline (p: pool):
+stt_ghost unit (deadline p) (fun () -> deadline p ** deadline p)
+
+
+
+
+
+//val small_inv (p: pool) (q: list task_elem) (c: int): vprop 
+
+
+// 0. init queue with task
+//val init_ghost_queue: stt_ghost pool emp (fun p -> inv p [] 0)
+
+
+
+
+
+// 1. enqueue task
+val spawn_task_ghost
+(p: pool)
+(q: list task_elem) (c: int)
+(t: task_elem)
+(#f: perm)
+: stt_ghost (secret_certificate p t)
+(small_inv p q c ** pts_to t._2 #three_quart None ** pool_alive f p)
+(fun _ -> small_inv p (t::q) c ** pool_alive f p)
+
+// 2. pop task todo
+val pop_task_ghost
+(p: pool)
+(t: task_elem)
+(q: list task_elem) (c: int)
+: stt_ghost (secret_certificate p t) 
+(small_inv p (t::q) c)
+(fun _ -> small_inv p q (c + 1) ** pts_to t._2 #three_quart None)
+
+(*
+val prove_task_ongoing
+  (#t: task_elem)
+  (#pos: nat)
+  (#v: option t._1)
+  (r:gmref)
+  (q: list task_elem) (c: int)
+  (w:certificate r t pos)
+: stt_ghost unit emp_inames
+(small_inv r q c ** pts_to t._2 #three_quart v)
+(fun () -> small_inv r q c ** pts_to t._2 #three_quart v ** pure (c > 0))
+
+val prove_ongoing_non_neg
+  (r: gmref)
+  (q: list task_elem) (c: int)
+: stt_ghost unit emp_inames
+(small_inv r q c)
+(fun () -> small_inv r q c ** pure (c >= 0))
+*)
+
+// 3. conclude a task
+val conclude_task_ghost
+(#t: task_elem)
+(#pos: nat)
+(p: pool)
+(q: list task_elem) (c: int)
+(x: t._1)
+(w: secret_certificate p t):
+stt_ghost unit 
+(small_inv p q c ** pts_to t._2 #three_quart (Some x))
+(fun () -> small_inv p q (c - 1)) //imp_vprop (c = 1 && L.length q = 0) (deadline r))
+
+val proof_promise (#t: task_elem) (#pos: nat)
+  (p: pool)
+  (w:secret_certificate p t)
+: stt_ghost unit 
+(deadline p)
+(fun () -> deadline p ** (exists* f v.
+                          pts_to t._2 #f v ** pure (Some? v)))
